Make more things work

SSA/Projects/InstCombine/ForStd.lean
@@ -1,4 +1,101 @@
 import Std.Data.BitVec
 
+open Std
+
 def ofBool : (Bool) -> Std.BitVec 1
  | c => if c then 1 else 0
+
+notation:50 x " ≤ᵤ " y => x ≤ y
+notation:50 x " <ᵤ " y => x < y
+notation:50 x " ≥ᵤ " y => x ≥ y 
+notation:50 x " >ᵤ " y => x > y
+
+notation:50 x " ≤ₛ " y => x ≤ y 
+notation:50 x " <ₛ " y => x < y
+notation:50 x " ≥ₛ " y => x ≥ y 
+notation:50 x " >ₛ " y => x > y
+
+instance {n} : ShiftLeft (BitVec n) := ⟨fun x y => x <<< y.toNat⟩
+
+instance {n} : ShiftRight (BitVec n) := ⟨fun x y => x >>> y.toNat⟩
+
+/--
+ If the condition is an i1 and it evaluates to 1, the instruction returns the first value argument; otherwise, it returns the second value argument.
+-/
+def select {w : Nat} (c : BitVec 1) (x y : BitVec w) : BitVec w :=
+  cond (c.toNat != 0) x y
+
+-- A lot of this should probably go to a differet file here and not Mathlib
+inductive Refinement {α : Type u} : Option α → Option α → Prop
+  | bothSome {x y : α } : x = y → Refinement (some x) (some y)
+  | noneAny {x? : Option α} : Refinement none x?
+
+theorem Refinement.some_some {α : Type u} {x y : α} :
+  Refinement (some x) (some y) ↔ x = y :=
+  ⟨by intro h; cases h; assumption, Refinement.bothSome⟩
+
+namespace Refinement
+
+theorem refl {α: Type u} : ∀ x : Option α, Refinement x x := by
+  intro x ; cases x
+  apply Refinement.noneAny
+  apply Refinement.bothSome; rfl
+
+theorem trans {α : Type u} : ∀ x y z : Option α, Refinement x y → Refinement y z → Refinement x z := by
+  intro x y z h₁ h₂
+  cases h₁ <;> cases h₂ <;> try { apply Refinement.noneAny } ; try {apply Refinement.bothSome; assumption}
+  rename_i x y hxy y h 
+  rw [hxy, h]; apply refl
+
+instance {α : Type u} [DecidableEq α] : DecidableRel (@Refinement α) := by
+  intro x y
+  cases x <;> cases y
+  { apply isTrue; exact Refinement.noneAny}
+  { apply isTrue; exact Refinement.noneAny }
+  { apply isFalse; intro h; cases h }
+  { rename_i val val'
+    cases (decEq val val')
+    { apply isFalse; intro h; cases h; contradiction } 
+    { apply isTrue; apply Refinement.bothSome; assumption }
+  }
+
+end Refinement
+
+infix:50 (priority:=low) " ⊑ " => Refinement
+
+/--
+The value produced is the unsigned integer quotient of the two operands.
+Note that unsigned integer division and signed integer division are distinct operations; for signed integer division, use ‘sdiv’.
+Division by zero is undefined behavior.
+-/
+def udiv? {w : Nat} (x y : BitVec w) : Option $ BitVec w :=
+  match y.toNat with
+    | 0 => none
+    | _ => some $ BitVec.ofNat w (x.toNat / y.toNat)
+
+/--
+The value produced is the signed integer quotient of the two operands rounded towards zero.
+Note that signed integer division and unsigned integer division are distinct operations; for unsigned integer division, use ‘udiv’.
+Division by zero is undefined behavior.
+Overflow also leads to undefined behavior; this is a rare case, but can occur, for example, by doing a 32-bit division of -2147483648 by -1.
+-/
+def sdiv? {w : Nat} (x y : BitVec w) : Option $ BitVec w := 
+  if y.toInt = 0 
+  then none
+  else 
+    let div := (x.toInt / y.toInt)
+    if div < 1 --2^w 
+      then some $ BitVec.ofInt w div
+      else none
+
+/--
+This instruction returns the unsigned integer remainder of a division. This instruction always performs an unsigned division to get the remainder.
+Note that unsigned integer remainder and signed integer remainder are distinct operations; for signed integer remainder, use ‘srem’.
+Taking the remainder of a division by zero is undefined behavior. 
+-/
+def urem? {w : Nat} (x y : BitVec w) : Option $ BitVec w :=
+  if y.toNat = 0 
+  then none
+  else some $ BitVec.ofNat w (x.toNat % y.toNat)
+
+instance : Coe Bool (BitVec 1) := ⟨ofBool⟩
